Replacing old decoding method with new decoding method which reads the output bitstring directly from the trellis rather than calculating it indirectly through the path taken back through the trellis.

ConvolutionalCodes/trellisScript.sml
@@ -235,74 +235,21 @@ Theorem best_origin_slow_def = cj 3 viterbi_trellis_slow
 Theorem viterbi_trellis_node_slow_def = cj 4 viterbi_trellis_slow
 
 (* -------------------------------------------------------------------------- *)
-(* Performs one step back through the trellis.                                *)
-(*                                                                            *)
-(* m: the state machine which generates the trellis                           *)
-(* bs: the bitstring being decoded                                            *)
-(* s: the state to step back from                                             *)
-(* t: the time-step to step back from                                         *)
-(*                                                                            *)
-(* Only valid for t > 0, since we can't step back at t = 0.                   *)
-(* -------------------------------------------------------------------------- *)
-(* Note: this requires generating the entire trellis up to this point, which  *)
-(* is slow. Repeatedly calling this function should therefore in theory be    *)
-(* less efficient than generating the trellis once and then stepping back     *)(* through the thing.                                                         *)
-(* -------------------------------------------------------------------------- *)
-Definition vd_step_back_def:
-  vd_step_back m bs s t =
-  let
-    trellis_row = viterbi_trellis_row m bs t;
-    trellis_node = EL s trellis_row
-  in
-    (THE trellis_node.prev_transition).origin
-End
-
-(* -------------------------------------------------------------------------- *)
-(* Returns the optimal path leading to state s at timestep t, with respect to *)
-(* the bitstring bs that we are trying to approximate.                        *)
-(*                                                                            *)
-(* Returns the path as a list of all states encountered along the path,       *)
-(* including the very first and last states, with the first element of this   *)
-(* list being the first state encountered in the path, and the last element   *)
-(* of this list being the last state encountered in the path.                 *)
+(* Decodes the input string bs with respect to the state machine m, assuming  *)
+(* we want to end at state s at time-step t.                                  *)
 (*                                                                            *)
 (* vd stands for Viterbi Decode                                               *)
 (* -------------------------------------------------------------------------- *)
-(* TODO: Repeatedly calling vd_step_back is slow, because it regenerates the  *)
-(* trellis at each step.                                                      *)
+(* TODO: In each step we call viterbi_trellis_row. This is slow, because it   *)
+(* regenerates all rows before it at each step.                               *)
 (* -------------------------------------------------------------------------- *)
-Definition vd_find_optimal_path_def:
-  vd_find_optimal_path m bs s 0 = [s] ∧
-  vd_find_optimal_path m bs s (SUC t) =
-  SNOC s (vd_find_optimal_path m bs (vd_step_back m bs s (SUC t)) t)
-End
-
-(* -------------------------------------------------------------------------- *)
-(* Added for legacy reasons. Do not use in new code. Phase out where possible.*)(* -------------------------------------------------------------------------- *)
-Definition vd_find_optimal_reversed_path_def:
-  vd_find_optimal_reversed_path m bs s t = REVERSE (vd_find_optimal_path m bs s t)
-End
-
-Definition get_num_errors_from_state_def:
-  get_num_errors_from_state m rs bs s = hamming_distance rs (vd_encode_from_state m bs s)
-End
-
-(* -------------------------------------------------------------------------- *)
-(* The number of errors present if we encoded the input bs with the state     *)(* machine m and compared it to the expected output rs.                       *)
-(* -------------------------------------------------------------------------- *)
-Definition get_num_errors_def:
-  get_num_errors m rs bs = get_num_errors_from_state m rs bs 0
-End
-
-Definition get_better_final_state_def:
-  get_better_final_state last_row s1 s2 = if (EL s1 last_row).num_errors < (EL s2 last_row).num_errors then s1 else s2
-End
-
-(* -------------------------------------------------------------------------- *)
-(* vd_find_optimal_path, but converted to code form                           *)
-(* -------------------------------------------------------------------------- *)
-Definition vd_find_optimal_code_def:
-  vd_find_optimal_code m bs s t = path_to_code m (vd_find_optimal_path m bs s t)
+Definition vd_decode_to_state_def:
+  vd_decode_to_state m bs s 0 = [] ∧
+  vd_decode_to_state m bs s (SUC t) =
+  let
+    prev_transition = best_origin m bs (viterbi_trellis_row m bs t) (SUC t) s;
+  in
+    SNOC (prev_transition).input (vd_decode_to_state m bs prev_transition.origin t)
 End
 
 (* -------------------------------------------------------------------------- *)
@@ -318,9 +265,20 @@ Definition vd_decode_def:
   let
     max_timestep = (LENGTH bs) DIV m.output_length;
     last_row = viterbi_trellis_row m bs max_timestep;
-    best_state = FOLDR (get_better_final_state last_row) 0 (COUNT_LIST m.num_states)
+    best_state = inargmin (λs. (EL s last_row).num_errors) (COUNT_LIST m.num_states)
   in
-    vd_find_optimal_code m bs best_state max_timestep
+    vd_decode_to_state m bs best_state max_timestep
+End
+
+Definition get_num_errors_from_state_def:
+  get_num_errors_from_state m rs bs s = hamming_distance rs (vd_encode_from_state m bs s)
+End
+
+(* -------------------------------------------------------------------------- *)
+(* The number of errors present if we encoded the input bs with the state     *)(* machine m and compared it to the expected output rs.                       *)
+(* -------------------------------------------------------------------------- *)
+Definition get_num_errors_def:
+  get_num_errors m rs bs = get_num_errors_from_state m rs bs 0
 End
 
 Theorem best_origin_is_valid[simp]:
@@ -524,71 +482,6 @@ Proof
   >> gvs[viterbi_trellis_node_slow_def]        
 QED
 
-Theorem vd_find_optimal_path_nonempty[simp]:
-  ∀m bs s t.
-    vd_find_optimal_path m bs s t ≠ []
-Proof
-  rpt strip_tac
-  >> Cases_on ‘t’ >> gvs[vd_find_optimal_path_def]
-QED
-
-Theorem vd_find_optimal_path_time_zero[simp]:
-  ∀m bs s t. vd_find_optimal_path m bs s 0 = [s]
-Proof
-  rpt strip_tac
-  >> EVAL_TAC
-QED
-
-Theorem vd_find_optimal_path_length[simp]:
-  ∀m bs s t.
-    LENGTH (vd_find_optimal_path m bs s t) = t + 1
-Proof
-  gen_tac
-  (* Induct over t *)
-  >> Induct_on ‘t’
-  >- (rpt strip_tac >> EVAL_TAC)
-  (* Expand out definitions *)
-  >> gvs[vd_find_optimal_path_def, vd_step_back_def]
-QED
-
-Theorem vd_find_optimal_path_last[simp]:
-  ∀m bs s t.
-    LAST (vd_find_optimal_path m bs s t) = s
-Proof
-  Induct_on ‘t’ >> rpt strip_tac >> gvs[]
-  >> gvs[vd_find_optimal_path_def]
-  >> gvs[vd_find_optimal_reversed_path_def]
-QED
-
-Theorem vd_find_optimal_path_suc:
-  ∀m bs s t.
-    vd_find_optimal_path m bs s (SUC t) = SNOC s (vd_find_optimal_path m bs (vd_step_back m bs s (SUC t)) t)
-Proof
-  rpt strip_tac
-  >> PURE_REWRITE_TAC[vd_find_optimal_path_def]
-  >> PURE_REWRITE_TAC[GSYM (cj 2 REVERSE_SNOC_DEF)]
-  >> AP_TERM_TAC
-  >> gvs[vd_find_optimal_reversed_path_def]
-QED
-
-Theorem vd_find_optimal_reversed_path_length[simp]:
-  ∀m bs s t.
-    LENGTH (vd_find_optimal_reversed_path m bs s t) = t + 1
-Proof
-  gvs[vd_find_optimal_reversed_path_def]
-QED
-
-(* -------------------------------------------------------------------------- *)
-(* This is already contained in the definition of                             *)
-(* vd_find_optimal_reversed_path, but it is good to automatically use it      *)
-(* -------------------------------------------------------------------------- *)
-Theorem vd_find_optimal_reversed_path_time_zero[simp]:
-  ∀m bs s.
-    vd_find_optimal_reversed_path m bs s 0 = [s]
-Proof
-  rpt strip_tac >> EVAL_TAC
-QED
-
 Theorem get_num_errors_from_state_append:
   ∀m rs bs bs' s.
     wfmachine m ∧
@@ -615,78 +508,25 @@ Proof
   >> gvs[vd_encode_state_def]
 QED
 
-Theorem vd_find_optimal_code_time_zero[simp]:
-  ∀m bs s. vd_find_optimal_code m bs s 0 = []
+Theorem vd_decode_to_state_time_zero[simp]:
+  ∀m bs s. vd_decode_to_state m bs s 0 = []
 Proof
   rpt strip_tac
-  >> gvs[vd_find_optimal_code_def]
+  >> gvs[vd_decode_to_state_def]
 QED
 
-Theorem vd_find_optimal_code_length[simp]:
+Theorem vd_decode_to_state_length[simp]:
   ∀m bs s t.
-    LENGTH (vd_find_optimal_code m bs s t) = t
+    LENGTH (vd_decode_to_state m bs s t) = t
 Proof
-  rpt strip_tac
-  >> gvs[vd_find_optimal_code_def]
+  Induct_on ‘t’ >> gvs[vd_decode_to_state_def]
 QED
-
-(* -------------------------------------------------------------------------- *)
-(* Theorem statement not designed by hand: identified after seeing what       *)
-(* happens when we expand out vd_find_optimal_code in order to remove the     *)
-(* SUC, intended for use in applying the inductive step.                      *)
-(* -------------------------------------------------------------------------- *)
-Theorem vd_find_optimal_code_suc:
-  ∀m bs s t.
-    vd_find_optimal_code m bs s (SUC t) = vd_find_optimal_code m bs (vd_step_back m bs s (SUC t)) t ⧺ [states_to_transition_input m (vd_step_back m bs s (SUC t))s] 
-Proof
-  gvs[vd_find_optimal_code_def]
-  >> gvs[vd_find_optimal_path_def]
-  >> gvs[vd_find_optimal_reversed_path_def]
-  >> gvs[GSYM vd_find_optimal_reversed_path_def]
-  >> gvs[GSYM vd_find_optimal_path_def]
-  >> gvs[path_to_code_append]
-  >> gvs[GSYM vd_find_optimal_code_def]
-QED
-
-(* -------------------------------------------------------------------------- *)
-(* Alternate definition that could be used for vd_find_optimal_code           *)
-(* -------------------------------------------------------------------------- *)
-Theorem vd_find_optimal_code_suc':
-  ∀m bs s t.
-    vd_find_optimal_code m bs s (SUC t) =
-    let
-      x = vd_step_back m bs s (SUC t)
-    in
-      vd_find_optimal_code m bs x t ⧺ [states_to_transition_input m x s]
-Proof
-  gvs[vd_find_optimal_code_def]
-  >> gvs[vd_find_optimal_path_def]
-  >> gvs[vd_find_optimal_reversed_path_def]
-  >> gvs[GSYM vd_find_optimal_reversed_path_def]
-  >> gvs[GSYM vd_find_optimal_path_def]
-  >> gvs[path_to_code_append]
-  >> gvs[GSYM vd_find_optimal_code_def]
-QED
-
-(* -------------------------------------------------------------------------- *)
-(* Alternate method to prove a theorem without having to re-write out the     *)
-(* entire statement of the theorem.                                           *)
-(* -------------------------------------------------------------------------- *)
-Theorem vd_find_optimal_code_suc'' =
-        “vd_find_optimal_code m bs s (SUC t)”
-          |> SCONV  [vd_find_optimal_code_def, vd_find_optimal_path_def,
-                     vd_find_optimal_reversed_path_def]
-          |> SRULE [GSYM vd_find_optimal_reversed_path_def,
-                    GSYM vd_find_optimal_path_def,
-                    path_to_code_append,
-                    GSYM vd_find_optimal_code_def]
-          |> GEN_ALL
 
 Theorem vd_decode_empty[simp]:
   ∀m. vd_decode m [] = []
 Proof
   rpt strip_tac
-  >> gvs[vd_decode_def, vd_find_optimal_code_def]
+  >> gvs[vd_decode_def]
 QED
 
 Theorem vd_decode_length[simp]:
@@ -812,25 +652,6 @@ Theorem is_reachable_viterbi_trellis_node_slow_prev_transition:
 Proof
   rpt strip_tac
   >> metis_tac[is_reachable_viterbi_trellis_node_slow_num_errors, viterbi_trellis_node_slow_prev_transition_num_errors]
-QED
-
-Theorem vd_step_back_is_valid[simp]:
-  ∀m bs s t.
-    wfmachine m ∧
-    s < m.num_states ∧
-    0 < t ∧
-    is_reachable m s t ⇒
-    vd_step_back m bs s t < m.num_states
-Proof
-  rpt strip_tac
-  >> gvs[vd_step_back_def]
-  >> Cases_on ‘t’ >> gvs[]
-  >> PURE_REWRITE_TAC[GSYM viterbi_trellis_node_no_prev_data_def]
-  >> gvs[GSYM viterbi_trellis_node_slow_viterbi_trellis_node_no_prev_data]
-  >> Cases_on ‘(viterbi_trellis_node_slow m bs s (SUC n)).prev_transition’
-  >- metis_tac[is_reachable_viterbi_trellis_node_slow_prev_transition]
-  >> gvs[]
-  >> gvs[viterbi_trellis_node_slow_def]
 QED
 
 Theorem best_origin_slow_get_num_errors_after_step_slow_infinity:
@@ -990,46 +811,17 @@ Proof
   >> gvs[viterbi_trellis_node_restrict_input]
 QED
 
-Theorem vd_step_back_restrict_input:
+Theorem vd_decode_to_state_restrict_input:
   ∀m bs s t n.
     t * m.output_length ≤ n ⇒
-    vd_step_back m (TAKE n bs) s t = vd_step_back m bs s t
-Proof
-  rpt strip_tac
-  >> gvs[vd_step_back_def]
-  >> gvs[viterbi_trellis_row_restrict_input]
-QED
-
-Theorem vd_step_back_restrict_input_apply:
-  ∀m bs s t.
-    vd_step_back m bs s t = vd_step_back m (TAKE (t * m.output_length) bs) s t
-Proof
-  gvs[vd_step_back_restrict_input]
-QED
-
-Theorem vd_find_optimal_code_restrict_input:
-  ∀m bs s t n.
-    t * m.output_length ≤ n ⇒
-    vd_find_optimal_code m (TAKE n bs) s t = vd_find_optimal_code m bs s t
+    vd_decode_to_state m (TAKE n bs) s t = vd_decode_to_state m bs s t
 Proof
   Induct_on ‘t’
   >- gvs[]
   >> rpt strip_tac
-  >> gvs[vd_find_optimal_code_suc]
-  >> REVERSE conj_tac
-  >- gvs[vd_step_back_restrict_input]
-  >> gvs[vd_step_back_restrict_input]
-  >> Cases_on ‘n = (SUC t) * m.output_length’ >> gvs[]
-  >> last_x_assum (fn th => DEP_PURE_ONCE_REWRITE_TAC [th])
-  >> gvs[]
-  >> gvs[ADD1]
-QED
-
-Theorem vd_find_optimal_code_restrict_input_apply:
-  ∀m bs s t.
-    vd_find_optimal_code m bs s t = vd_find_optimal_code m (TAKE (t * m.output_length) bs) s t
-Proof
-  gvs[vd_find_optimal_code_restrict_input]
+  >> ‘t * m.output_length ≤ n’ by gvs[ADD1]
+  >> gvs[vd_decode_to_state_def]
+  >> gvs[best_origin_restrict_input, viterbi_trellis_row_restrict_input]
 QED
 
 Theorem get_num_errors_after_step_slow_restrict_input:
@@ -1075,21 +867,19 @@ Proof
 QED
 
 (* -------------------------------------------------------------------------- *)
-(* Alternate definition of the step_back function which uses the slow trellis *)
-(* code                                                                       *)
+(* Version of is_reachable_get_num_errors_after_step_slow which can be used   *)
+(* as a rewrite from get_num_errors_after_step_slow to is_reachable. The      *)
+(* other theorem cannot be used in that way even after applying GSYM, because *)
+(* the left hand side is negated.                                             *)
 (* -------------------------------------------------------------------------- *)
-Theorem vd_step_back_def_slow:
+Theorem get_num_errors_after_step_slow_is_reachable:
   ∀m bs s t.
     wfmachine m ∧
     s < m.num_states ⇒
-    vd_step_back m bs s t = (THE (viterbi_trellis_node_slow m bs s t).prev_transition).origin
+    (get_num_errors_after_step_slow m bs t (best_origin_slow m bs t s) = INFINITY ⇔ ¬is_reachable m s t)
 Proof
   rpt strip_tac
-  >> gvs[vd_step_back_def]
-  >> Cases_on ‘t’ >> gvs[]
-  >- (gvs[viterbi_trellis_node_slow_def]
-      >> EVAL_TAC >> Cases_on ‘s’ >> gvs[])
-  >> gvs[viterbi_trellis_node_slow_viterbi_trellis_node_no_prev_data]
+  >> metis_tac[is_reachable_get_num_errors_after_step_slow]
 QED
 
 (* -------------------------------------------------------------------------- *)
@@ -1263,51 +1053,6 @@ Proof
       >> EVAL_TAC)
 QED
 
-(* -------------------------------------------------------------------------- *)
-(* test_path: [F; T; T; F; T; T; T; T; F; F; T; F]                            *)
-(*                                                                            *)
-(*   0 -> 0/00 -> 0                                                           *)
-(*     -> 1/11 -> 1                                                           *)
-(*   1 -> 0/11 -> 2                                                           *)
-(*     -> 1/00 -> 3                                                           *)
-(*   2 -> 0/10 -> 0                                                           *)
-(*     -> 1/01 -> 1                                                           *)
-(*   3 -> 0/01 -> 2                                                           *)
-(*     -> 1/10 -> 3                                                           *)
-(*                                                                            *)
-(* 0  1  2  3  3  3  4                -  0  0  2  2  02 0                     *)
-(* -  1  2  2  3  3  4                -  0  0  0  02 2  0                     *)
-(* -  -  2  2  2  5  4                -  -  1  1  1  13 13                    *)
-(* -  -  2  3  4  3  3                -  -  1  3  13 1  3                     *)
-(*    FT TF TT TT FF TF                  FT TF TT TT FF TF                    *)
-(*                                                                            *)
-(* Starting at state 0, t=6: [0, 0, 0, 2, 1, 0, 0]                            *)
-(*                               .. 2, 1, 0, 0, 0]                            *)
-(*                                                                            *)
-(*                                                                            *)
-(* Starting at state 1, t=4: [1, 0, 2, 1, 0]                                  *)
-(*                            .. 2, 1, 0, 0]                                  *)
-(*                                                                            *)
-(* Starting at state 2, t=4: [2, 1, 0, 0, 0]                                  *)
-(*                                                                            *)
-(* Starting at state 3, t=6; [3, 3, 1, 0, 2, 1, 0]                            *)
-(*                                  .. 2, 1, 0, 0]                            *)
-(* -------------------------------------------------------------------------- *)
-Theorem vd_find_optimal_reversed_path_test:
-  let
-    result1 = (vd_find_optimal_reversed_path example_state_machine test_path 0 6);
-    result2 = (vd_find_optimal_reversed_path example_state_machine test_path 1 4);
-    result3 = (vd_find_optimal_reversed_path example_state_machine test_path 2 4);
-    result4 = (vd_find_optimal_reversed_path example_state_machine test_path 3 6);
-  in
-    (result1 = [0;0;0;2;1;0;0] ∨ result1 = [0;0;2;1;0;0;0]) ∧
-    (result2 = [1;0;2;1;0] ∨ result2 = [1;2;1;0;0]) ∧
-    (result3 = [2;1;0;0;0]) ∧
-    (result4 = [3;3;1;0;2;1;0] ∨ result4 = [3;3;1;2;1;0;0])
-Proof
-  EVAL_TAC
-QED
-
 (*Theorem vd_find_optimal_reversed_path_eval:
   let
     result1 = (vd_find_optimal_reversed_path example_state_machine test_path 0 6);
@@ -1400,6 +1145,59 @@ Proof
   >> EVAL_TAC
 QED
 
+(* -------------------------------------------------------------------------- *)
+(* test_path: [F; T; T; F; T; T; T; T; F; F; T; F]                            *)
+(*                                                                            *)
+(*   Transitions:                                                             *)
+(*   0 -> 0/00 -> 0                                                           *)
+(*     -> 1/11 -> 1                                                           *)
+(*   1 -> 0/11 -> 2                                                           *)
+(*     -> 1/00 -> 3                                                           *)
+(*   2 -> 0/10 -> 0                                                           *)
+(*     -> 1/01 -> 1                                                           *)
+(*   3 -> 0/01 -> 2                                                           *)
+(*     -> 1/10 -> 3                                                           *)
+(*                                                                            *)
+(* Trellis num errors:                Trellis previous state:                 *)
+(* 0  1  2  3  3  3  4                -  0  0  2  2  02 0                     *)
+(* -  1  2  2  3  3  4                -  0  0  0  02 2  0                     *)
+(* -  -  2  2  2  5  4                -  -  1  1  1  13 13                    *)
+(* -  -  2  3  4  3  3                -  -  1  3  13 1  3                     *)
+(*    FT TF TT TT FF TF                  FT TF TT TT FF TF                    *)
+(*                                                                            *)
+(* Examples of optimal paths back through trellis:                            *)
+(* State 0, t=6: [0, 0, 0, 2, 1, 0, 0]                                        *)
+(*                   .. 2, 1, 0, 0, 0]                                        *)
+(* State 1, t=4: [1, 0, 2, 1, 0]                                              *)
+(*                .. 2, 1, 0, 0]                                              *)
+(* State 2, t=4: [2, 1, 0, 0, 0]                                              *)
+(* State 3, t=6; [3, 3, 1, 0, 2, 1, 0]                                        *)
+(*                      .. 2, 1, 0, 0]                                        *)
+(*                                                                            *)
+(* Examples of optimal decoded paths to given states:                         *)
+(* State 0, t=6: [F, T, F, F, F, F]                                           *)
+(*               [F, F, T, F, ... ]                                           *)
+(* State 1, t=4: [T, F, F, T]                                                 *)
+(*               [F, T, F ...]                                                *)
+(* State 2, t=4: [F, F, T, F]                                                 *)
+(* State 3, t=6: [T, F, F, T, T, T]                                           *)
+(*               [F, T, F, ... ]                                              *)
+(* -------------------------------------------------------------------------- *)
+Theorem vd_decode_to_state_test:
+  let
+    result1 = (vd_decode_to_state example_state_machine test_path 0 6);
+    result2 = (vd_decode_to_state example_state_machine test_path 1 4);
+    result3 = (vd_decode_to_state example_state_machine test_path 2 4);
+    result4 = (vd_decode_to_state example_state_machine test_path 3 6);
+  in
+    (result1 = [F; T; F; F; F; F] ∨ result1 = [F; F; T; F; F; F]) ∧
+    (result2 = [T; F; F; T] ∨ result2 = [F; T; F; T]) ∧
+    (result3 = [F; F; T; F]) ∧
+    (result4 = [T; F; F; T; T; T] ∨ result4 = [F; T; F; T; T; T])
+Proof
+  EVAL_TAC
+QED
+
 (*Theorem vd_decode_eval:
   let
     decoded_path = vd_decode example_state_machine test_path;
@@ -1412,35 +1210,5 @@ QED
 Proof
   EVAL_TAC
 QED*)
-
-(* -------------------------------------------------------------------------- *)
-(* Version of is_reachable_get_num_errors_after_step_slow which can be used   *)
-(* as a rewrite from get_num_errors_after_step_slow to is_reachable. The      *)
-(* other theorem cannot be used in that way even after applying GSYM, because *)
-(* the left hand side is negated.                                             *)
-(* -------------------------------------------------------------------------- *)
-Theorem get_num_errors_after_step_slow_is_reachable:
-  ∀m bs s t.
-    wfmachine m ∧
-    s < m.num_states ⇒
-    (get_num_errors_after_step_slow m bs t (best_origin_slow m bs t s) = INFINITY ⇔ ¬is_reachable m s t)
-Proof
-  rpt strip_tac
-  >> metis_tac[is_reachable_get_num_errors_after_step_slow]
-QED
-
-Theorem is_reachable_vd_step_back:
-  ∀m bs s t.
-    wfmachine m ∧
-    s < m.num_states ∧
-    is_reachable m s (SUC t) ⇒
-    is_reachable m (vd_step_back m bs s (SUC t)) t
-Proof
-  rpt strip_tac
-  >> gvs[vd_step_back_def_slow]
-  >> gvs[viterbi_trellis_node_slow_def]
-  >> gvs[get_num_errors_after_step_slow_is_reachable]
-  >> gvs[is_reachable_best_origin_slow]
-QED
 
 val _ = export_theory();
